\documentclass[12pt]{article}
\usepackage{amsmath}  % For advanced math typesetting
\usepackage{amsfonts} % For math fonts
\usepackage{amssymb}  % For additional symbols
\usepackage{graphicx} % For including images
\usepackage{geometry} % For page layout
\usepackage{fancyhdr} % For header and footer
\usepackage{setspace} % For line spacing
\usepackage{hyperref} % For hyperlinks
\usepackage{titlesec} % For customizing section titles
\usepackage{tikz} % For drawing
\usepackage{braket} % For braket notation

\geometry{a4paper, margin=1in}

% Header and Footer
\pagestyle{fancy}
\fancyhf{}
\fancyhead[L]{Proof of Similarity Transformation relation}
\fancyhead[R]{\thepage}
\fancyfoot[C]{\thepage}

% Title Formatting
\titleformat{\section}{\Large\bfseries}{\thesection}{1em}{}
\titleformat{\subsection}{\large\bfseries}{\thesubsection}{1em}{}

% Title Page
\title{\textbf{Proof of Similarity Transformation relation}}
\author{
    MohamadAli Khajeian\footnote{khajeian@ut.ac.ir} \\ 
    \small \textit{Faculty of Engineering Sciences, University of Tehran, Iran} \\ 
}
\date{\today}

\begin{document}

\maketitle

\begin{abstract}
    This document presents the Proof of Similarity Transformation relation.
\end{abstract}

\section*{Proof}

Assume we have state vector $\ket{\psi}$ and we want to transform two orthonormal basis to each other $\{\ket{u_{i}}\} \rightleftarrows \{\ket{v_{j}}\}$

\begin{equation}
    \label{1}
    \ket{\psi}_{u} = \sum_{i} c_{i}\ket{u_{i}}, \quad c_{i} = \braket{u_{i}|\psi}
\end{equation}
\begin{equation}
    \label{2}
    \ket{\psi}_{v} = \sum_{j} d_{j}\ket{v_{j}}, \quad d_{j} = \braket{v_{j}|\psi}
\end{equation}
Let's start with $\{\ket{u_{i}}\} \rightarrow \{\ket{v_{j}}\}$
\begin{equation*}
    d_{j} = \braket{v_{j}|\psi} = \braket{v_{j}| \hat{\textnormal{I}} | \psi} = \braket{v_{j}| \big( \sum_{i} |u_{i}\rangle \langle u_{i}|\big) | \psi}
    = \sum_{i} \braket{v_{j}|u_{i}}\braket{u_{i}|\psi}
\end{equation*}
According to \ref{1} and $\braket{v_{j}|u_{i}} = S_{ji}$ 
\begin{equation}
    d_{j} = \sum_{i} \braket{v_{j}|u_{i}}c_{i} = \sum_{i} S_{ji}c_{i}
\end{equation}
Thus $S$ is our Similarity Matrix, so we can say
\begin{equation}
    \ket{\psi}_{v} = S\ket{\psi}_{u}
\end{equation}
We can repeat this for $\{\ket{v_{j}}\} \rightarrow \{\ket{u_{i}}\}$
\begin{equation*}
    c_{i} = \braket{u_{i}|\psi} = \braket{u_{i}| \hat{\textnormal{I}} | \psi} = \braket{u_{i}| \big( \sum_{j} |v_{j}\rangle \langle v_{j}|\big) | \psi}
    = \sum_{j} \braket{u_{i}|v_{j}}\braket{v_{j}|\psi}
\end{equation*}
According to \ref{2} and $\braket{u_{i}|v_{j}} = \braket{v_{j}|u_{i}}^{*} = S_{ji}^{*}$ 
\begin{equation}
    c_{i} = \sum_{j} \braket{u_{i}|v_{j}}d_{j} = \sum_{j} S_{ji}^{*}d_{j}
\end{equation}
So we have
\begin{equation}
    \ket{\psi}_{u} = S^{\dagger}\ket{\psi}_{v}
\end{equation}
\\
Now suppose we want to transform the matrix representation of an operator in one basis like $\hat{\textnormal{A}}^{u}$ to representation of that operator in another basis
like $\hat{\textnormal{A}}^{v}$
\begin{equation}
    \label{7}
    \hat{\textnormal{A}}^{u} = \sum_{i,j}\textnormal{A}_{ij}^{u}|u_{j}\rangle \langle u_{i}|, \quad \textnormal{A}_{ij}^{u} = \braket{u_{i}|\hat{\textnormal{A}}|u_{j}}
\end{equation}
\begin{equation}
    \label{8}
    \hat{\textnormal{A}}^{v} = \sum_{k,l}\textnormal{A}_{kl}^{v}|v_{k}\rangle \langle v_{l}|, \quad \textnormal{A}_{kl}^{v} = \braket{v_{k}|\hat{\textnormal{A}}|v_{l}}
\end{equation}
Let's start with $\textnormal{A}_{kl}^{v}$
\begin{equation*}
    \textnormal{A}_{kl}^{v} = \braket{v_{k}|\hat{\textnormal{A}}|v_{l}} = \braket{v_{k}|\hat{\textnormal{I}}\hat{\textnormal{A}}\hat{\textnormal{I}}|v_{l}}
    = \braket{v_{k}|\big(\sum_{i} |u_{i}\rangle \langle u_{i}| \big)\hat{\textnormal{A}}\big(\sum_{j} |u_{j}\rangle \langle u_{j}| \big)|v_{l}} \\
\end{equation*}
\begin{equation*}
    = \sum_{i,j} \braket{v_{k}|u_{i}} \braket{u_{i}| \hat{\textnormal{A}} | u_{j}} \braket{u_{j}| v_{l}}
\end{equation*}
According to \ref{7}, $\braket{v_{k}|u_{i}} = S_{ki}$ and $\braket{u_{j}| v_{l}} = S_{lj}^{*}$,
we can write
\begin{equation}
    \textnormal{A}_{kl}^{v} = \sum_{i,j} \braket{v_{k}|u_{i}} \braket{u_{i}| \textnormal{A} | u_{j}} \braket{u_{j}| v_{l}} = \sum_{i,j} S_{ki} \textnormal{A}_{ij}^{u} S_{lj}^{*}
\end{equation}
Thus $S$ is our Similarity Matrix, so we can say
\begin{equation}
    \hat{\textnormal{A}}^{v} = S\hat{\textnormal{A}}^{u}S^{\dagger}
\end{equation}
We can repeat this for $\textnormal{A}_{ij}^{u}$
\begin{equation*}
    \textnormal{A}_{ij}^{u} = \braket{u_{i}|\hat{\textnormal{A}}|u_{j}} = \braket{u_{i}|\hat{\textnormal{I}}\hat{\textnormal{A}}\hat{\textnormal{I}}|u_{j}}
    = \braket{u_{i}|\big(\sum_{k} |v_{k}\rangle \langle v_{k}| \big)\hat{\textnormal{A}}\big(\sum_{l} |v_{l}\rangle \langle v_{l}| \big)|u_{j}} \\
\end{equation*}
\begin{equation*}
    = \sum_{k,l} \braket{u_{i}|v_{k}} \braket{v_{k}| \hat{\textnormal{A}} | v_{l}} \braket{v_{l}| u_{j}}
\end{equation*}
According to \ref{8}, $\braket{u_{i}|v_{k}} = S_{ki}^{*}$ and $\braket{u_{l}| v_{j}} = S_{lj}$,
we can write
\begin{equation}
    \textnormal{A}_{ij}^{u} = \sum_{k,l} \braket{u_{i}|v_{k}} \braket{v_{k}| \hat{\textnormal{A}} | v_{l}} \braket{v_{l}| u_{j}} = \sum_{k,l} S_{ki}^{*} \textnormal{A}_{kl}^{v} S_{lj}
\end{equation}
Thus $S$ is our Similarity Matrix, so we can say
\begin{equation}
    \hat{\textnormal{A}}^{u} = S^{\dagger}\hat{\textnormal{A}}^{v}S
\end{equation}
\end{document}
